rpc/impl.v
@@ -5,7 +5,7 @@ From iris.algebra Require Import agree auth csum gset gmap excl frac.
 From iris.algebra Require Import max_prefix_list.
 From iris.heap_lang Require Import notation proofmode.
 From cryptis Require Import lib term cryptis primitives tactics.
-From cryptis Require Import role iso_dh.
+From cryptis Require Import role iso_dh conn.
 
 Set Implicit Arguments.
 Unset Strict Implicit.
@@ -17,184 +17,43 @@ Section Impl.
 
 Variable N : namespace.
 
-Definition session_key : val := λ: "cs",
-  Snd "cs".
-
 Definition connect : val := λ: "c" "skA" "vkB",
-  let: "session_key" :=
-    do_until (λ: <>, initiator (N.@"conn".@"auth") "c" "skA" "vkB") in
-  let: "timestamp" := ref #0%nat in
-  let: "m" := senc (Tag $ N.@"conn".@"init") "session_key" (TInt 0) in
-  send "c" "m";;
-  ("timestamp", "session_key").
+  Conn.connect (N.@"rpc".@"auth") "c" "skA" "vkB".
 
-Definition listen : val := λ: "c",
-  do_until (λ: <>,
-    let: "req" := responder_wait "c" in
-    let: "vkA" := Snd "req" in
-    bind: "kt" := is_key "vkA" in
-    guard: "kt" = repr Open in
-    SOME "req").
+Definition listen : val := λ: "c", Conn.listen "c".
 
 Definition confirm : val := λ: "c" "skB" "req",
-  let: "ga" := Fst "req" in
-  let: "vkA" := Snd "req" in
-  let: "sk" := do_until
-    (λ: <>, responder_accept (N.@"conn".@"auth") "c" "skB" "ga" "vkA") in
-  do_until (λ: <>,
-    let: "m" := recv "c" in
-    sdec (Tag $ N.@"conn".@"init") "sk" "m");;
-  let: "timestamp" := ref #0%nat in
-  ("timestamp", "sk").
+  Conn.confirm (N.@"rpc".@"auth") "c" "skB" "req".
 
-Definition timestamp : val := λ: "cs",
-  let: "timestamp" := Fst "cs" in
-  !"timestamp".
+Definition call (s : string) : val := λ: "c" "cs" "ts",
+  Conn.write (Tag $ N.@s.@"call") "c" "cs" "ts";;
+  Conn.read  (Tag $ N.@s.@"resp") "c" "cs".
 
-Definition tick : val := λ: "cs",
-  let: "timestamp" := Fst "cs" in
-  "timestamp" <- (!"timestamp" + #1).
-
-Definition write N : val := λ: "c" "cs" "ts",
-  let: "n"  := timestamp "cs" in
-  let: "sk" := session_key "cs" in
-  let: "m"  := term_of_list (tint "n" :: "ts") in
-  let: "m"  := senc N "sk" "m" in
-  send "c" "m".
-
-Definition open' : val := λ: "N" "n" "m",
-  bind: "m" := untag "N" "m" in
-  bind: "ts" := list_of_term "m" in
-  match: "ts" with
-    NONE => NONE
-  | SOME "ts" =>
-    bind: "n'" := to_int (Fst "ts") in
-    guard: "n" = "n'" in
-    SOME (Snd "ts")
-  end.
-
-Definition make_handler_def (p : namespace * expr) : expr :=
-  let N := p.1 in
-  let: "handler" := p.2 in
-  λ: "n" "m",
-    bind: "ts" := open' (Tag N) "n" "m" in
-    "handler" "ts".
-
-Definition make_handler_aux : base.seal make_handler_def. by eexists _. Qed.
-Definition make_handler := unseal make_handler_aux.
-Lemma make_handler_eq : make_handler = make_handler_def.
-Proof. exact: seal_eq. Qed.
-
-Lemma subst_make_handler var v p :
-  subst var v (make_handler p) =
-  make_handler (p.1, subst var v p.2).
-Proof.
-rewrite make_handler_eq /make_handler_def.
-case: p => [N' handler] /=.
-case: decide => [[_ not_shadow_handler]|shadow_handler //].
-case: decide => [[_ not_shadow_n]|shadow_n //].
-case: decide => [[_ not_shadow_m]|shadow_m //].
-rewrite decide_False; last congruence.
-rewrite decide_False; last congruence.
-case: decide => [[_ not_shadow_ts]|shadow_ts //].
-rewrite decide_False; last congruence.
-by rewrite decide_False; last congruence.
-Qed.
-
-Fixpoint make_handlers (handlers : list (namespace * expr)) : expr :=
-  match handlers with
-  | [] => []%E
-  | handler :: handlers => (make_handler handler :: make_handlers handlers)%E
-  end.
-
-Lemma subst_make_handlers var v handlers :
-  subst var v (make_handlers handlers) =
-  make_handlers (map (λ p, (p.1, subst var v p.2)) handlers).
-Proof.
-elim: handlers=> [|p handlers IH] //=.
-by rewrite -IH -subst_make_handler.
-Qed.
-
-Definition select_inner_body : val := rec: "loop" "ts" "m" "handlers" :=
-  match: "handlers" with
-    NONE => NONE
-  | SOME "handlers" =>
-    let: "handler" := Fst "handlers" in
-    let: "handlers" := Snd "handlers" in
-    match: "handler" "ts" "m" with
-      NONE => "loop" "ts" "m" "handlers"
-    | SOME "res" => SOME "res"
-    end
-  end.
-
-Definition select_outer_body : val := λ: "c" "cs" "handlers",
-  let: "ts" := timestamp "cs" in
-  let: "sk" := session_key "cs" in
-  do_until (λ: <>,
-    let: "m" := recv "c" in
-    bind: "m" := open (key Open "sk") "m" in
-    select_inner_body "ts" "m" "handlers"
-  ).
-
-Definition select_def (c cs : expr) handlers : expr :=
-  select_outer_body c cs (make_handlers handlers).
-
-Definition select_aux : base.seal select_def. by eexists _. Qed.
-Definition select := unseal select_aux.
-Lemma select_eq : select = select_def. Proof. exact: seal_eq. Qed.
-
-Definition read N : val :=
-  let handlers := [(N, (λ: "ts", SOME "ts")%E)] in
-  λ: "c" "cs", select "c" "cs" handlers.
-
-Lemma subst_select var v c cs handlers :
-  subst var v (select c cs handlers) =
-  select
-    (subst var v c) (subst var v cs)
-    (map (λ p, (p.1, subst var v p.2)) handlers).
-Proof.
-by rewrite select_eq /select /= subst_make_handlers.
-Qed.
-
-Definition free : val := λ: "c" "cs",
-  let: "timestamp" := Fst "cs" in
-  Free "timestamp".
+Definition handle (s : string) : val := λ: "c" "f",
+  Conn.handle (Tag $ N.@s.@"call")
+    (λ: "cs" "ts",
+      match: "f" "ts" with
+        SOME "res" => Conn.write (Tag (N.@s.@"resp")) "c" "cs" "res"
+      | NONE => Conn.write (Tag (N.@"rpc".@"error")) "c" "cs" [TInt 0]
+      end;;
+      #true).
 
 Definition close : val := λ: "c" "cs",
-  write (Tag $ N.@"conn".@"close") "c" "cs" [];;
-  read (N.@"conn".@"ack_close") "c" "cs";;
-  free "c" "cs".
+  Conn.write (Tag $ N.@"rpc".@"close".@"call") "c" "cs" [TInt 0];;
+  Conn.read  (Tag $ N.@"rpc".@"close".@"resp") "c" "cs";;
+  Conn.free "c" "cs".
 
-Definition handle_close N : val := λ: "c" "cs" "req",
-  write (Tag $ N.@"conn".@"ack_close") "c" "cs" [TInt 0];;
-  free "c" "cs";;
-  SOME #false.
+Definition handle_close : val := λ: "c",
+  Conn.handle (Tag $ N.@"rpc".@"close".@"call")
+    (λ: "cs" "ts",
+      Conn.write (Tag (N.@"rpc".@"close".@"resp")) "c" "cs" [TInt 0];;
+      Conn.free "c" "cs";;
+      #false).
 
-Definition handle_loop : val :=
-  rec: "loop" "c" "cs" "handlers" :=
-    if: select_outer_body "c" "cs" "handlers" then
-      "loop" "c" "cs" "handlers"
-    else #().
-
-Definition handle_def c cs handlers :=
-  let handle_close :=
-    make_handler (N.@"conn".@"close", handle_close N "c" "cs") in
-  (λ: "c" "cs" "handlers",
-    handle_loop "c" "cs" (handle_close :: "handlers"))%V
-  c cs (make_handlers handlers).
-
-Definition handle_aux : base.seal handle_def. by eexists _. Qed.
-Definition handle := unseal handle_aux.
-Lemma handle_eq : handle = handle_def. Proof. exact: seal_eq. Qed.
-
-Lemma subst_handle var v c cs handlers :
-  subst var v (handle c cs handlers) =
-  handle
-    (subst var v c) (subst var v cs)
-    (map (λ p, (p.1, subst var v p.2)) handlers).
-Proof.
-by rewrite handle_eq /handle_def /= subst_make_handlers.
-Qed.
+Definition server : val := rec: "loop" "c" "cs" "handlers" :=
+  let: "cont" := Conn.select "c" "cs" (handle_close "c" :: "handlers") in
+  if: "cont" then "loop" "c" "cs" "handlers"
+  else #().
 
 End Impl.
 
