rpc/proofs.v
@@ -5,7 +5,7 @@ From iris.algebra Require Import agree auth csum gset gmap excl frac.
 From iris.algebra Require Import max_prefix_list.
 From iris.heap_lang Require Import notation proofmode.
 From cryptis Require Import lib term gmeta cryptis primitives tactics.
-From cryptis Require Import role iso_dh.
+From cryptis Require Import role iso_dh conn.
 From cryptis.rpc Require Import impl props.
 
 Set Implicit Arguments.
@@ -18,57 +18,14 @@ Import Props Impl.
 
 Section Proofs.
 
-Context `{!cryptisGS Σ, !heapGS Σ, !connGS Σ}.
+Context `{!cryptisGS Σ, !heapGS Σ, !Conn.connGS Σ}.
 Notation iProp := (iProp Σ).
 
-Implicit Types (cs : state).
+Implicit Types (cs : Conn.state).
 Implicit Types kI kR kS t : term.
 Implicit Types n : nat.
 Implicit Types γ : gname.
 Implicit Types v : val.
-
-(* MOVE *)
-Lemma connected_public_key' kI kR cs n n0 kt :
-  connected' kI kR cs false n n0 -∗
-  public (TKey kt (si_key cs)) -∗
-  ◇ compromised_session (cs_role cs) cs.
-Proof.
-iIntros "conn #p_k".
-iPoseProof "conn" as "(_ & _ & #sess & rel & _)".
-iDestruct "sess" as "(#? & #s_key & #sess)".
-iPoseProof (senc_key_compromised_keyI with "s_key p_k") as "{p_k} p_k".
-iPoseProof (senc_key_compromised_keyE with "s_key p_k") as "{p_k} >p_k".
-by iApply session_compromised.
-Qed.
-(* /MOVE *)
-
-Lemma public_sencE N rl si m φ :
-  public (TSeal (TKey Seal (si_key si)) (Spec.tag (Tag N) m)) -∗
-  seal_pred N φ -∗
-  wf_sess_info rl si -∗
-  release_token (si_share_of rl si) -∗
-  ▷ □ (compromised_session rl si ∗ public m ∨ φ (si_key si) m).
-Proof.
-iIntros "#p_m #Nφ #(_ & s_key & sess) rel".
-iDestruct (public_TSealE with "[//] [//]") as "{p_m} [[p_key p_m]|p_m]".
-- iPoseProof ("s_key" with "p_key") as "{p_key} >p_key".
-  iPoseProof (session_compromised with "[//] p_key rel") as "#>?".
-  iModIntro. iLeft. iModIntro. by do 2!iSplit => //.
-- iDestruct "p_m" as "[#p_m _]". by eauto.
-Qed.
-
-Lemma or_sep1 (P Q R : iProp) : P ∨ Q -∗ P ∨ R -∗ P ∨ Q ∗ R.
-Proof.
-iIntros "[?|?] [?|?]"; eauto. iRight. by iFrame.
-Qed.
-
-Lemma or_sep2 (P Q R : iProp) :
-  Persistent P →
-  P ∨ Q ∗ R ⊢ (P ∨ Q) ∗ (P ∨ R).
-Proof.
-iIntros "% [#?|[Q R]]"; first by iSplitR; eauto.
-by iSplitL "Q"; eauto.
-Qed.
 
 Lemma wp_connect P N c kI kR n :
   channel c -∗
@@ -76,67 +33,24 @@ Lemma wp_connect P N c kI kR n :
   ctx N -∗
   sign_key kI -∗
   public (TKey Open kR) -∗
-  {{{ client_disconnected N kI kR n ∗ (failure kI kR ∨ P) }}}
+  {{{ client_disconnected N kI kR n ∗ (Conn.failure kI kR ∨ P) }}}
     Impl.connect N c kI (TKey Open kR)
   {{{ cs, RET (repr cs);
-      connected kI kR cs n ∗
-      (compromised_session Init cs ∨ P) ∗
-      client_token N kI kR cs }}}.
+      client_connected N kI kR cs n ∗
+      (compromised_session Init cs ∨ P) }}}.
 Proof.
-iIntros "#? #? #? #? #? % !> ((#server_clock & dis) & HP) post".
-iPoseProof (or_sep1 with "dis HP") as "H".
-rewrite bi.or_alt. iDestruct "H" as "(%failed & dis)".
-wp_lam. wp_pure _ credit:"c1". wp_pure _ credit:"c2".
-wp_pures. wp_bind (do_until _).
-iAssert (if failed then failure kI kR else True)%I as "#?".
-{ by case: failed. }
-iCombine "dis post c1 c2" as "post". iApply (wp_frame_wand with "post").
-wp_apply wp_do_until'. iModIntro.
-wp_pures.
-wp_apply (wp_initiator _ failed with "[//] [//] [] [] []") => //.
-- by iApply ctx_iso_dh_ctx.
-- case: failed => //. by eauto.
-iIntros "%res resP".
-case: res=> [kS|] /=; last by eauto.
-iDestruct "resP"
-  as "(%si & <- & %e_kR & <- & #m_kS & #sess & #comp & rel & token)".
-case: e_kR => <- {kR}.
-iRight. iExists _. iSplit => //.
-iIntros "(dis & post & c1 & c2)".
-wp_pures.
-wp_alloc ts as "ts". wp_pures.
-pose cs := State si ts Init.
-iMod (term_meta_set' (N := isoN.@"beginning") n with "token")
-  as "[#beginning token]"; first by solve_ndisj.
-iPoseProof (term_token_drop (↑isoN.@"end") with "token")
-  as "end"; first by solve_ndisj.
-iAssert (|={⊤}=> compromised_session Init si ∨ conn_ready N si n ∗ P)%I
-  with "[dis]" as ">conn_ready".
-{ case: failed.
-  - iModIntro. iLeft. by iApply "comp".
-  - iDestruct "dis" as "[dis P]".
-    iAssert (|={⊤}=> conn_ready N si n)%I with "[dis]" as ">#?".
-    { iApply (escrowI with "dis"). iApply term_token_switch. }
-    by eauto. }
-rewrite or_sep2. iDestruct "conn_ready" as "[#conn_ready P]".
-wp_apply wp_senc. wp_pures. wp_apply wp_send => //.
-{ iDestruct "conn_ready" as "[(_ & p_k & _)|conn_ready]".
-  - iApply public_TSealIP.
-    + by iApply public_TKey; eauto.
-    + by rewrite public_tag public_TInt.
-  - iApply public_TSealIS.
-    + by rewrite minted_TKey.
-    + by iApply ctx_init.
-    + iModIntro. iExists si. rewrite public_TInt.
-      do 2!iSplit => //. iExists n. by eauto.
-    + by rewrite minted_TInt.
-    + rewrite public_TInt. by eauto. }
-wp_pures. iApply ("post" $! cs).
-iSplitR "end P".
-- iExists 0, n. iFrame. iModIntro. do 5!iSplit => //.
-  + iSplit => //. iSplit => //. by iApply senc_key_si_key.
-  + by eauto.
-- iFrame. by eauto.
+iIntros "#? #? #? #? #? % !> (clock & P) post".
+iPoseProof (Conn.or_sep1 with "clock P") as "P".
+wp_lam; wp_pures.
+iPoseProof (Props.ctx_conn_ctx with "[//]") as "?".
+iApply wp_fupd.
+wp_apply (Conn.wp_connect with "[//] [//] [//] [//] [//] P").
+iIntros "%cs (connected & P & rel & token)".
+iMod (term_meta_set (isoN.@"conn".@"beg") n with "token")
+  as "#meta"; first solve_ndisj.
+iDestruct (Conn.or_sep2 with "P") as "[clock P]".
+iApply "post". iFrame.
+iModIntro. iExists n. iSplit => //. by iPureIntro; lia.
 Qed.
 
 Lemma wp_listen N c :
@@ -149,17 +63,8 @@ Lemma wp_listen N c :
       public ga ∗ public (TKey Open skA) }}}.
 Proof.
 iIntros "#? #? #? % !> _ post".
-wp_lam. iApply (wp_frame_wand with "post"). wp_pures.
-wp_apply wp_do_until'.
-iModIntro. wp_pures.
-wp_apply wp_responder_wait; eauto.
-iIntros "%ga %vkA #(p_ga & #p_vkA)".
-wp_pures. wp_apply wp_is_key.
-case: Spec.is_keyP => [kt skA -> {vkA}|_]; wp_pures; last by eauto.
-case: bool_decide_reflect => [e|_]; wp_pures; last by eauto.
-case: kt => // in e *.
-iModIntro. iRight. iExists _. iSplit => //.
-iIntros "post". iApply "post". by eauto.
+wp_lam. iApply Conn.wp_listen => //.
+by iApply Props.ctx_conn_ctx.
 Qed.
 
 Lemma wp_confirm P N c skA skB ga n :
@@ -168,577 +73,246 @@ Lemma wp_confirm P N c skA skB ga n :
   ctx N -∗
   {{{ public ga ∗ public (TKey Open skA) ∗ sign_key skB ∗
       server_disconnected N skA skB n ∗
-      (failure skA skB ∨ P) }}}
+      (Conn.failure skA skB ∨ P) }}}
     confirm N c skB (ga, TKey Open skA)%V
   {{{ cs, RET (repr cs);
-      ⌜cs_role cs = Resp⌝ ∗
-      ⌜si_init cs = skA⌝ ∗
-      ⌜si_resp cs = skB⌝ ∗
-      connected skA skB cs n ∗
-      (compromised_session Resp cs ∨ P) ∗
-      server_token N cs }}}.
+      server_connected N skA skB cs n ∗
+      (compromised_session Resp cs ∨ P) }}}.
 Proof.
 iIntros "#? #ctx #? !> %Φ (#p_ga & #p_vkA & #sign_skB & dis & P) post".
-iPoseProof (or_sep1 with "dis P") as "dis".
-rewrite bi.or_alt. iDestruct "dis" as "(%failed & dis)".
-wp_lam. wp_pures.
-iAssert (if failed then failure skA skB else True)%I
-  as "#?".
-{ by case: failed. }
-wp_bind (do_until _).
-iApply (wp_frame_wand with "post").
-iApply (wp_frame_wand with "dis").
-iApply wp_do_until'. iIntros "!>".
-wp_pures.
-iPoseProof (ctx_iso_dh_ctx with "[//]") as "#?".
-iApply (wp_responder_accept _ failed).
-{ do !iSplit => //. case: failed => //. by eauto. }
-iIntros "!> %osi res". case: osi => [si|]; last by eauto.
-iDestruct "res" as "(%e & <- & #m_k & #sess & #comp & rel & token)".
-case: e => -> {skA}.
-iRight. iExists _. iSplit => //.
-iIntros "dis post".
-wp_pures. wp_bind (do_until _).
-iApply (wp_frame_wand with "post").
-iApply (wp_frame_wand with "token").
-iCombine "rel dis" as "I". iRevert "I".
-iApply wp_do_until.
-iIntros "!> [rel dis]".
-wp_pures. wp_apply wp_recv => //. iIntros "%m #p_m". wp_pures.
-wp_sdec m; last first.
-{ iModIntro. iLeft. by iFrame. }
-iModIntro. iRight. iExists _. iSplit => //. iIntros "token post".
-wp_pures. wp_alloc ts as "ts". 
-iPoseProof (ctx_init with "[//]") as "#?".
-iPoseProof (senc_key_si_key with "ctx m_k") as "#?".
-iPoseProof (public_sencE _ Resp with "p_m [//] [] rel") as "{p_m} #p_m".
-{ do !iSplit => //. }
-wp_pure _.
-iMod (term_meta_set' (N:=isoN.@"beginning") n with "token")
-  as "[#beginningB token]"; first by solve_ndisj.
-rewrite (term_token_difference _ (↑isoN.@"begin")); last by solve_ndisj.
-iDestruct "token" as "[begin token]".
-iAssert (|={⊤}=>
-  compromised_session Resp si ∨ P ∗
-  term_meta (si_init_share si) (isoN.@"beginning") n ∗
-  ∃ n0, clock N (si_init si) (si_resp si) n0 ∗
-        clock N (si_init si) (si_resp si) n0)%I
-  with "[dis begin]" as ">con".
-{ iDestruct "p_m" as "#[[? _]|inv]"; first by eauto.
-  iDestruct "inv" as "(%si' & %e & _ & inv)".
-  rewrite -(session_agree e) {si' e}.
-  iDestruct "inv" as "(%beginning & clock_ready & beginning & conn_ready)".
-  case: failed.
-  { iModIntro. iLeft. by iApply "comp". }
-  iDestruct "dis" as "[dis P]".
-  iDestruct "dis" as "[[-> never]|clockB]".
-  { iMod (escrowE with "clock_ready never") as ">clockB"; eauto.
-    iMod (escrowE with "conn_ready begin") as ">clockA"; eauto.
-    iPoseProof (clock_agree with "clockA clockB") as "->".
-    iModIntro. iRight. by iFrame. }
-  iMod (escrowE with "conn_ready begin") as ">clockA"; eauto.
-  iPoseProof (clock_agree with "clockA clockB") as "->".
-  iModIntro. iRight. by iFrame. }
-rewrite 2!or_sep2. iDestruct "con" as "(P & (#? & ?))".
-wp_pures. iApply ("post" $! (State si ts Resp)).
-iModIntro. iSplit => //=. iFrame. iSplit => //.
-do !iSplit => //. iExists n. by do !iSplit => //.
-Qed.
-
-Lemma wp_timestamp kI kR cs b n n0 :
-  {{{ connected' kI kR cs b n n0 }}}
-    timestamp (repr cs)
-  {{{ RET #n; connected' kI kR cs b n n0 }}}.
-Proof.
-rewrite /timestamp.
-iIntros "%Φ Hn post".
-iDestruct "Hn" as "(% & % & #? & ? & ? & #?)".
-wp_pures. wp_load. iApply "post". iFrame.
-iModIntro. by eauto 10.
-Qed.
-
-Lemma wp_tick kI kR cs n :
-  {{{ connected kI kR cs n }}}
-    tick (repr cs)
-  {{{ RET #(); connected kI kR cs (S n) }}}.
-Proof.
-iIntros "%Ψ (%n' & %n0 & -> & #? & Hn) post".
-iDestruct "Hn" as "(% & % & #? & ? & ? & #?)".
-rewrite /tick; wp_pures; wp_load; wp_store.
-iApply "post".
-rewrite (_ : (n' + 1)%Z = (S n')%nat :> Z); last by lia.
-iFrame; eauto 10.
-Qed.
-
-Lemma wp_session_key cs :
-  {{{ True }}}
-    session_key (repr cs)
-  {{{ RET (repr (si_key cs)); True }}}.
-Proof.
-rewrite /session_key.
-iIntros "%Φ _ post". wp_pures. iApply "post".
-iModIntro. by iFrame.
-Qed.
-
-Lemma wp_write' kI kR cs b n1 n0 N c ts φ :
-  channel c -∗
-  seal_pred N (conn_pred φ) -∗
-  ([∗ list] t ∈ ts, public t) -∗
-  compromised_session (cs_role cs) cs ∨ □ φ kI kR cs (n1 + n0) ts -∗
-  {{{ connected' kI kR cs b n1 n0 }}}
-    write (Tag N) c (repr cs) (repr ts)
-  {{{ RET #(); connected' kI kR cs b n1 n0 }}}.
-Proof.
-iIntros "#chan #pred #p_ts #inv !> %Φ conn post".
-iAssert (⌜kI = si_init cs⌝ ∗ ⌜kR = si_resp cs⌝)%I as "#[-> ->]".
-{ by iDestruct "conn" as "(<- & <- & _)". }
-wp_lam. wp_pures. wp_apply (wp_timestamp with "[$]").
-iIntros "conn". wp_pures.
-wp_apply wp_session_key => //. iIntros "_".
-wp_pures. wp_apply wp_tint. wp_list. wp_term_of_list.
-wp_pures. wp_apply wp_senc. wp_pures.
-iAssert (wf_sess_info (cs_role cs) cs) as "#wf".
-{ by iDestruct "conn" as "(? & ? & ? & ?)". }
-iAssert (compromised_session (cs_role cs) cs ∨
-           term_meta (si_init_share cs) (isoN.@"beginning") n0)%I
-  as "#beginning".
-{ by iDestruct "conn" as "(? & ? & ? & ? & ? & ?)". }
-wp_apply (wp_send with "[//] [#]").
-{ iDestruct "inv" as "[(_ & ? & _)|#inv]".
-  { iModIntro. iApply public_TSealIP.
-    + by iApply public_TKey; eauto.
-    + rewrite public_tag public_of_list /= public_TInt. by eauto. }
-  iDestruct "beginning" as "[(_ & ? & _)|beginning]".
-  { iModIntro. iApply public_TSealIP.
-    + by iApply public_TKey; eauto.
-    + rewrite public_tag public_of_list /= public_TInt. by eauto. }
- iModIntro. iApply public_TSealIS; eauto.
- - rewrite minted_TKey. by iDestruct "wf" as "(? & ? & ?)".
- - iModIntro. iExists cs, n1, ts, n0. do !iSplit => //.
- - iApply public_minted.
-   rewrite public_of_list /= public_TInt. by eauto.
- - rewrite public_of_list /= public_TInt. by eauto. }
-by iApply "post".
-Qed.
-
-Lemma wp_write kI kR cs n N c ts φ :
-  channel c -∗
-  seal_pred N (conn_pred φ) -∗
-  ([∗ list] t ∈ ts, public t) -∗
-  compromised_session (cs_role cs) cs ∨ □ φ kI kR cs n ts -∗
-  {{{ connected kI kR cs n }}}
-    write (Tag N) c (repr cs) (repr ts)
-  {{{ RET #(); connected kI kR cs n }}}.
-Proof.
-iIntros "#chan #pred #p_ts #inv !> %Φ conn post".
-iDestruct "conn" as "(%n' & %n0 & -> & #? & conn)".
-wp_apply (wp_write' with "[//] [//] p_ts inv conn").
-iIntros "conn". iApply "post". iExists n', n0. by eauto.
-Qed.
-
-Lemma wp_select_inner_body_aux φ v1 v2 (handlers : list val) (Φ : val → iProp) :
-  ([∗ list] handler ∈ handlers,
-    (φ -∗ WP (handler : val) v1 v2 {{ v',
-           ⌜v' = NONEV⌝ ∗ φ ∨
-           ∃ r, ⌜v' = SOMEV r⌝ ∗ Φ r }}))%I -∗
-  φ -∗ WP select_inner_body v1 v2 (repr handlers) {{ v',
-      ⌜v' = NONEV⌝ ∗ φ ∨
-      ∃ r, ⌜v' = SOMEV r⌝ ∗ Φ r }}.
-Proof.
-rewrite /= repr_list_unseal.
-iIntros "wp_handlers inv".
-iLöb as "IH" forall (handlers).
-wp_rec; case: handlers=> [|handler handlers]; wp_pures; first by eauto.
-rewrite /=. iDestruct "wp_handlers" as "[wp_handler wp_handlers]".
-iSpecialize ("wp_handler" with "inv").
-iSpecialize ("IH" with "wp_handlers").
-wp_bind (handler _ _); iApply (wp_wand with "wp_handler").
-iIntros "%v' [[-> inv] | (%r & -> & post)]"; wp_pures.
-- by iApply "IH".
-- iRight. iExists r. by iFrame.
-Qed.
-
-Lemma wp_select_inner_body Φ φ v1 v2 (handlers : list val) Ψ :
-  ([∗ list] handler ∈ handlers,
-     (φ -∗ WP (handler : val) v1 v2 {{ v,
-       ⌜v = NONEV⌝ ∗ φ ∨
-       ∃ r, ⌜v = SOMEV r⌝ ∗ Φ r }}))%I -∗
-  (φ -∗ Ψ NONEV) -∗
-  (∀ r, Φ r -∗ Ψ (SOMEV r)) -∗
-  φ -∗
-  WP select_inner_body v1 v2 (repr handlers) {{ Ψ }}.
-Proof.
-iIntros "wp post1 post2 inv".
-iApply (wp_wand with "[wp inv] [post1 post2]").
-- by iApply (wp_select_inner_body_aux φ v1 v2 handlers Φ with "[wp] inv").
-- iIntros "%res [[-> ?]|(%r & -> & ?)]".
-  + by iApply "post1".
-  + by iApply "post2".
-Qed.
-
-Lemma wp_open' N φ kI kR cs n n0 m :
-  {{{ seal_pred N (conn_pred φ) ∗
-      connected' kI kR cs false n n0 ∗
-      public (TSeal (TKey Seal (si_key cs)) m) }}}
-    open' (Tag N) #n m
-  {{{ res, RET res;
-      connected' kI kR cs false n n0 ∗
-      (⌜res = NONEV⌝ ∨
-       ∃ ts, ⌜res = SOMEV (repr ts)⌝ ∗
-             ([∗ list] t ∈ ts, public t) ∗
-             □ (compromised_session (cs_role cs) cs ∨ φ kI kR cs (n + n0) ts)) }}}.
-Proof.
-iIntros "%Φ (#Φ & conn & #p_m) post".
-rewrite /open'.
-wp_pure _ credit:"c1".
-wp_pure _ credit:"c2".
-wp_pures.
-wp_untag m; wp_pures; last by iApply "post"; eauto.
-wp_list_of_term m; wp_pures; last by iApply "post"; eauto.
-case: m => [|t ts].
-{ rewrite repr_list_unseal. wp_pures. by iApply "post"; eauto. }
-rewrite repr_list_unseal /= -repr_list_unseal.
-wp_pures. wp_apply wp_to_int.
-case: Spec.to_intP => [n' ->|_]; wp_pures; last by iApply "post"; eauto.
-case: bool_decide_reflect => [[<-]|ne]; wp_pures; last by iApply "post"; eauto.
-iPoseProof (public_sencE with "p_m [//] [#] [conn]") as "{p_m} #p_m".
-- by iDestruct "conn" as "(? & ? & ? & ? & ?)".
-- by iDestruct "conn" as "(? & ? & ? & ? & ?)".
-iAssert (□ ▷ (([∗ list] t ∈ ts, public t) ∗
-           (compromised_session (cs_role cs) cs ∨ φ kI kR cs (n + n0) ts)))%I
-  as "#H".
-{ iDestruct "conn" as "(<- & <- & ? & ? & ? & #beginning)".
-  iIntros "!> !>".
-  iDestruct "p_m" as "#[[comp p_m]|inv]".
-  - rewrite public_of_list /=. iDestruct "p_m" as "[_ p_m]".
-    iSplit => //. by eauto.
-  - iDestruct "inv"
-      as "(%si & %n'' & %ts' & %n0' & %e_k & %e_m & p_ts & beginning' & ?)".
-    move/session_agree: e_k => <- {si}.
-    case/Spec.of_list_inj: e_m => e_n <-.
-    have <-: n = n'' by lia.
-    iSplit => //.
-    iDestruct "beginning" as "[?|beginning]"; eauto.
-    iPoseProof (term_meta_agree with "beginning beginning'") as "->".
-    iRight. by eauto. }
-iMod (lc_fupd_elim_later_pers with "c1 H") as "{H} #[p_ts inv_ts]".
-iModIntro. iApply "post". iFrame. iRight. by eauto.
-Qed.
-
-Definition make_handler_post φ ψ kI kR cs (handler : val) : iProp :=
-  □ ∀ n1 n0 (m : term),
-    public (TSeal (TKey Seal (si_key cs)) m) -∗
-    term_meta (cs_share cs) (isoN.@"beginning") n0 -∗
-    connected' kI kR cs false n1 n0 -∗
-    φ (n1 + n0) -∗
-    WP handler #n1 m {{ v,
-      ⌜v = NONEV⌝ ∗ connected' kI kR cs false n1 n0 ∗ φ (n1 + n0) ∨
-      ∃ r, ⌜v = SOMEV r⌝ ∗ ψ (n1 + n0) r }}.
-
-Definition handler_correct_gen φ ψ kI kR cs handler : iProp :=
-  WP handler.2 {{ f,
-    ∃ Ψ, seal_pred handler.1 (conn_pred Ψ) ∗
-    □ ∀ n ts,
-      {{{ connected kI kR cs n ∗ φ n ∗
-          ▷ ([∗ list] t ∈ ts, public t) ∗
-          □ ▷ (compromised_session (cs_role cs) cs ∨ Ψ kI kR cs n ts) }}}
-        (f : val) (repr ts)
-      {{{ v, RET v;
-         ⌜v = NONEV⌝ ∗ connected kI kR cs n ∗ φ n ∨
-         ∃ r, ⌜v = SOMEV r⌝ ∗ ψ n r }}}
-  }}%I.
-
-Lemma wp_make_handler φ ψ kI kR cs (handler : namespace * expr) :
-  handler_correct_gen φ ψ kI kR cs handler -∗
-  WP make_handler handler {{ make_handler_post φ ψ kI kR cs }}.
-Proof.
-case: handler => N handler /=; iIntros "wp".
-rewrite make_handler_eq /make_handler_def. wp_pures.
-wp_bind handler. iApply (wp_wand with "wp").
-iIntros "%v_handler #(%φ' & #? & #wp)". wp_pures.
-iIntros "!> !> %n1 %n0 %m #p_m #beg conn inv". wp_pures.
-wp_apply (wp_open' with "[$conn]"); eauto.
-iIntros "%res (conn & [->|(%ts & -> & #p_ts & #inv_ts)])"; wp_pures.
-{ iLeft. by iFrame. }
-wp_apply ("wp" with "[$inv conn]").
-{ iFrame. iSplit; eauto. }
-iIntros "%res [(-> & conn & inv)|?]"; last by eauto.
-iLeft. iFrame. iSplit => //.
-iDestruct "conn" as "(%n1' & %n0' & %e & #beg' & conn)".
-iPoseProof (term_meta_agree with "beg beg'") as "<-".
-by have <- : n1 = n1' by lia.
-Qed.
-
-Lemma wp_make_handlers φ ψ kI kR cs handlers :
-  ([∗ list] handler ∈ handlers,
-    handler_correct_gen φ ψ kI kR cs handler) -∗
-  WP make_handlers handlers {{ v',
-    ∃ handlers : list val, ⌜v' = repr handlers⌝ ∗
-      [∗ list] handler ∈ handlers,
-        make_handler_post φ ψ kI kR cs handler }}.
-Proof.
-rewrite /= !repr_list_unseal.
-elim: handlers=> [|[N handler] handlers IH] //=.
-  iIntros "_". wp_pures. iModIntro. iExists []. by rewrite /=.
-iIntros "[wp_handler wp_handlers]".
-wp_bind (make_handlers _).
-iPoseProof (IH with "wp_handlers") as "wp_handlers". clear IH.
-iApply (wp_wand with "wp_handlers [wp_handler]").
-iIntros "%v' (%handlers' & -> & #Hhandlers')".
-wp_bind (make_handler _).
-iApply (wp_wand with "[wp_handler] [Hhandlers']").
-{ iApply (wp_make_handler _ _ _ _ _ (N, handler) with "wp_handler"). }
-iIntros "%f #wp_f". wp_lam; wp_pures.
-iExists (f :: handlers'). iSplitR => //=.
-iModIntro. iSplit => //.
-Qed.
-
-Lemma wp_select_outer_body φ ψ (c : val) kI kR cs (handlers : list val) :
-  channel c -∗
-  ([∗ list] handler ∈ handlers,
-    make_handler_post φ ψ kI kR cs handler) -∗
-  ∀ n n0,
-  term_meta (cs_share cs) (isoN.@"beginning") n0 -∗
-  connected' kI kR cs false n n0 -∗
-  φ (n + n0) -∗
-  WP select_outer_body c (repr cs) (repr handlers) {{ ψ (n + n0) }}.
-Proof.
-iIntros "#chan_c #wps %n %n0 #beg conn inv".
-wp_lam. wp_pures. wp_apply (wp_timestamp with "conn"). iIntros "conn".
-wp_pures. wp_apply wp_session_key => //. iIntros "_".
-wp_pures. iCombine "conn inv" as "I". iRevert "I". iApply wp_do_until.
-iIntros "!> I". wp_pures. wp_bind (recv _). iApply wp_recv => //.
-iIntros "%m #p_m". wp_pures.
-wp_apply wp_key.
-wp_bind (open _ _). iApply wp_open.
-case: Spec.openP; last by wp_pures; iLeft; iFrame.
-move=> _ {}m [<-] ->. wp_pures.
-iApply (wp_select_inner_body (ψ (n + n0)) with "[] [] [] I").
-- iApply (big_sepL_impl with "wps").
-  iIntros "!> %k %handler _ #Hhandler (conn & inv)" => //.
-  by iApply ("Hhandler" with "p_m [//] conn inv").
-- iIntros "(?&?)". iLeft. by iFrame.
-- iIntros "%r Hr". iRight. iExists r. by eauto.
-Qed.
-
-Lemma wp_select
-  φ ψ (c : val) kI kR cs (handlers : list (namespace * expr)) :
-  channel c -∗
-  ([∗ list] handler ∈ handlers,
-    handler_correct_gen φ ψ kI kR cs handler) -∗
-  ∀ n, connected kI kR cs n -∗
-  φ n -∗
-  WP select c (repr cs) handlers {{ ψ n }}.
-Proof.
-rewrite select_eq /select_def.
-iIntros "#chan_c wps %n (%n' & %n0 & -> & #beg & conn) inv".
-wp_bind (make_handlers _). iApply (wp_wand with "[wps]").
-{ wp_apply (wp_make_handlers with "wps"). }
-iIntros "%res (%v_handlers & -> & #wps)".
-by wp_apply (wp_select_outer_body with "[] [] [] conn inv").
-Qed.
-
-Lemma wp_read N c kI kR cs n φ :
-  channel c -∗
-  seal_pred N (conn_pred φ) -∗
-  {{{ connected kI kR cs n }}}
-    read N c (repr cs)
-  {{{ ts, RET (repr (ts : list term));
-      connected kI kR cs n ∗
-      ([∗ list] t ∈ ts, public t) ∗
-      □ (compromised_session (cs_role cs) cs ∨ φ kI kR cs n ts) }}}.
-Proof.
-iIntros "#? #NΦ !> %Ψ conn post".
-wp_lam. wp_pures. rewrite !subst_select /=.
-wp_apply (wp_select
-  (λ n, (∀ ts, connected kI kR cs n ∗
-          ([∗ list] t ∈ ts, public t) ∗
-          □ (compromised_session (cs_role cs) cs ∨ φ kI kR cs n ts) -∗
-          Ψ (repr ts)))%I with "[] [] conn post") => //.
-rewrite /= /handler_correct_gen /=. iSplit => //. wp_pures.
-iModIntro. iExists _; iSplit; eauto.
-iModIntro. clear n.
-iIntros "%n %ts !> %Φ (conn & post1 & #p_ts & #inv_ts) post2".
-wp_pures. iModIntro.
-iApply "post2". iRight. iExists _. iSplit => //.
-iApply "post1". iFrame. by eauto.
-Qed.
-
-Lemma wp_free (c : val) cs n :
-  {{{ cs_ts cs ↦ #n }}}
-    free c (repr cs)
-  {{{ RET #(); True }}}.
-Proof.
-iIntros "%Φ ts post".
+iPoseProof (Conn.or_sep1 with "dis P") as "dis".
 wp_lam; wp_pures.
-wp_free.
-by iApply "post".
+iPoseProof (Props.ctx_conn_ctx with "[//]") as "?".
+iApply wp_fupd.
+wp_apply (Conn.wp_confirm (server_clock N skA skB n ∗ P)
+           with "[//] [//] [//] [$dis]").
+{ by eauto. }
+iIntros "%cs (conn & dis & rel & token)".
+iMod (term_meta_set (isoN.@"conn".@"beg") n with "token")
+  as "#meta"; first solve_ndisj.
+iDestruct (Conn.or_sep2 with "dis") as "[dis P]".
+iApply "post". iFrame. iExists n. iModIntro. iSplit; eauto. iPureIntro. lia.
+Qed.
+
+Lemma wp_call N s φ ψ kI kR c cs n (ts : list term) :
+  {{{ channel c ∗ cryptis_ctx ∗ ctx N ∗
+      ([∗ list] t ∈ ts, public t) ∗
+      rpc_pred N s φ ψ ∗
+      client_connected N kI kR cs n ∗
+      (compromised_session Init cs ∨ φ kI kR cs n ts) }}}
+    call N s c (repr cs) (repr ts)
+  {{{ ts', RET (repr ts');
+      client_connected N kI kR cs (S n) ∗
+      (compromised_session Init cs ∨ ψ kI kR cs n ts') ∗
+      ([∗ list] t ∈ ts', public t) }}}.
+Proof.
+iIntros "%Φ (#? & #? & #? & #p_ts & #(? & ?) & conn & inv) post".
+iDestruct "conn" as "(%n1 & %n0 & -> & conn & #beg & rel & clock)".
+wp_lam; wp_pures.
+wp_apply (Conn.wp_write with "[//] [] [] [$conn clock inv]"); eauto.
+{ iDestruct "inv" as "[?|inv]"; first by eauto.
+  iDestruct "clock" as "[?|clock]"; first by eauto.
+  iRight. iExists n0. by iFrame. }
+iIntros "conn". wp_pures.
+wp_apply (Conn.wp_read with "[//] [] [$conn $rel]"); eauto.
+iIntros "%ts' (conn & rel & p_ts' & inv)".
+iApply "post". iFrame. iDestruct "inv" as "[#inv|inv]".
+{ iSplitR; eauto. iExists n0. iSplit; first by iPureIntro; lia.
+  iSplit => //. by eauto. }
+iDestruct "inv" as "(%n0' & #beg' & clock & inv)".
+iPoseProof (term_meta_agree with "beg beg'") as "<-".
+iFrame. iExists n0.
+have -> : S (n0 + n1) = (n0 + S n1)%nat by lia.
+iFrame. by eauto.
+Qed.
+
+Definition handler Φ kI kR cs N (handler : val) : iProp :=
+  Conn.handler
+    (λ n1 m, ∃ n0,
+      ⌜m = n1⌝ ∗
+      term_meta (si_resp_share cs) (isoN.@"conn".@"beg") n0 ∗
+      Φ (n0 + n1) ∗
+      (compromised_session Resp cs ∨ server_clock N kI kR (n0 + n1)))%I
+    (λ n1 m r, ∃ n0,
+      ⌜m = n1⌝ ∗
+      term_meta (si_resp_share cs) (isoN.@"conn".@"beg") n0 ∗
+      (⌜r = #true⌝ ∗
+       Φ (S (n0 + n1)) ∗
+       Conn.connected kI kR Resp cs (S n1) (S n1) ∗
+       (compromised_session Resp cs ∨ server_clock N kI kR (S (n0 + n1))) ∗
+       release_token (si_resp_share cs) ∨
+       ⌜r = #false⌝ ∗
+       Φ (n0 + n1) ∗
+       (compromised_session Resp cs ∨ server_clock N kI kR (n0 + n1)) ∗
+       released (si_resp_share cs)))%I
+    kI kR Resp cs handler.
+
+Lemma wp_handle Φ N s φ₁ φ₂ kI kR c cs (f : val) :
+  {{{
+    channel c ∗
+    rpc_pred N s φ₁ φ₂ ∗
+    ctx N ∗
+    □ (∀ n (ts : list term),
+      {{{ ▷ ([∗ list] t ∈ ts, public t) ∗
+          ▷ (compromised_session Resp cs ∨ φ₁ kI kR cs n ts) ∗
+          Φ n }}}
+        f (repr ts)
+      {{{ ts', RET (repr ts');
+          match ts' with
+          | Some ts' => ([∗ list] t ∈ ts', public t) ∗
+                        (compromised_session Resp cs ∨ φ₂ kI kR cs n ts')
+          | None => True
+          end ∗
+          Φ (S n) }}})
+  }}}
+    handle N s c f
+  {{{ h, RET h; handler Φ kI kR cs N h }}}.
+Proof.
+iIntros "%Ψ (#chan_c & (#? & #?) & #ctx & #wp_f) post".
+iPoseProof (ctx_error with "[//]") as "#?".
+wp_lam; wp_pures.
+iApply (wp_wand with "[] post"). clear Ψ.
+iApply Conn.wp_handle; last first.
+{ iIntros "!> %h wp". iApply "wp". }
+iSplit => //.
+iIntros "!> %n1 %m %ts !> %Ψ (conn & rel & I & #p_ts & inv_ts) post".
+iDestruct "I" as "(%n0 & -> & #begS & I & clock)". wp_pures.
+iAssert (|==>
+           compromised_session Resp cs ∨
+           server_clock N kI kR (S (n0 + n1)) ∗
+           φ₁ kI kR cs (n0 + n1) ts ∗
+           term_meta (si_init_share cs) (isoN.@"conn".@"beg") n0 ∗
+           client_clock N kI kR (S (n0 + n1)))%I
+    with "[clock inv_ts]" as ">H".
+{ iDestruct "clock" as "[?|clockS]"; first by eauto.
+  iDestruct "inv_ts" as "[?|inv_ts]"; first by eauto.
+  iDestruct "inv_ts" as "(%n0' & #begC & clockC & inv)".
+  iMod (clock_update with "clockC clockS") as "(%e_n' & clockS & clockC)".
+  have <- : n0 = n0' by lia.
+  iModIntro. iRight. by iFrame. }
+iPoseProof (Conn.or_sep2 with "H") as "[clockS H]".
+iPoseProof (Conn.or_sep2 with "H") as "[inv clockC]".
+wp_apply ("wp_f" with "[$]"). iIntros "%ts' (inv_ts' & inv)".
+case: ts' => [ts'|]; wp_pures; last first.
+{ wp_list.
+  wp_apply (Conn.wp_write with "[//] [] [] [$conn]") => //.
+  { by rewrite /= public_TInt. }
+  { by iRight. }
+  iIntros "conn". wp_pures.
+  iApply "post". iModIntro. iExists n0. do !iSplit => //. iLeft. by iFrame. }
+iDestruct "inv_ts'" as "(#p_ts' & inv_ts')".
+wp_apply (Conn.wp_write with "[//] [] [] [inv_ts' clockC $conn]") => //.
+{ iDestruct "inv_ts'" as "[?|inv_ts']"; first by eauto.
+  iDestruct "clockC" as "[?|[#begC clockC]]"; first by eauto.
+  iRight. iExists n0. iFrame.
+  have -> : n0 + S n1 = S (n0 + n1) by lia. by iFrame. }
+iIntros "conn". wp_pures. iApply "post". iModIntro.
+iExists n0. do !iSplit => //. iFrame. iLeft. by iFrame.
+Qed.
+
+Lemma wp_handle_close Φ N c kI kR cs :
+  {{{ channel c ∗ ctx N }}}
+    handle_close N c
+  {{{ h, RET h; handler Φ kI kR cs N h }}}.
+Proof.
+iIntros "%Ψ (#chan_c & #ctx) post". wp_lam; wp_pures.
+iApply (wp_wand with "[] post"). clear Ψ.
+wp_apply Conn.wp_handle; last first.
+{ iIntros "% wp". iApply "wp". }
+iPoseProof (ctx_close with "ctx") as "#?".
+iPoseProof (ctx_ack_close with "ctx") as "#?".
+iSplit => //.
+iIntros "!> %n1 %m %ts !> %Ψ (conn & rel & inv & #p_ts & inv_ts) post".
+iDestruct "inv" as "(%n0 & -> & #begS & inv & clockS)". wp_pures.
+iAssert (|==>
+           compromised_session Resp cs ∨
+           server_clock N kI kR (n0 + n1) ∗
+           term_meta (si_init_share cs) (isoN.@"conn".@"beg") n0 ∗
+           client_clock N kI kR (n0 + n1))%I
+    with "[clockS inv_ts]" as ">H".
+{ iDestruct "clockS" as "[?|clockS]"; first by eauto.
+  iDestruct "inv_ts" as "[?|inv_ts]"; first by eauto.
+  iDestruct "inv_ts" as "(%n0' & #begC & clockC)".
+  iPoseProof (clock_agree with "clockC clockS") as "%e_n'".
+  have <- : n0 = n0' by lia.
+  iModIntro. iRight. by iFrame. }
+wp_pures.
+iPoseProof (Conn.or_sep2 with "H") as "[clockS clockC]".
+iMod (release with "rel") as "#rel".
+wp_list.
+wp_apply (Conn.wp_write with "[//] [] [] [clockC $conn]") => //.
+- by rewrite /= public_TInt.
+- iDestruct "clockC" as "[?|[#begC clockC]]"; first by eauto.
+  iRight. iExists n0. iFrame. by eauto.
+iIntros "conn". wp_pures. wp_apply (Conn.wp_free with "[$conn]").
+iIntros "_". wp_pures. iApply "post".
+iExists n0. iModIntro. do !iSplit => //.
+iFrame. iRight. iFrame. by eauto.
+Qed.
+
+Lemma wp_server Φ N kI kR c cs n handlers :
+  {{{ channel c ∗ ctx N ∗
+      server_connected N kI kR cs n ∗ Φ n ∗
+      [∗ list] h ∈ handlers, handler Φ kI kR cs N h }}}
+    server N c (repr cs) (repr handlers)
+  {{{ RET #(); ∃ n', server_disconnected N kI kR n' ∗ Φ n' }}}.
+Proof.
+iLöb as "IH" forall (n).
+iIntros "%Ψ (#chan_c & #ctx & conn & inv & #handlers) post".
+iDestruct "conn" as "(%n1 & %n0 & -> & conn & #beg & rel & clockS)".
+iPoseProof (Conn.connected_keyE with "conn") as "#(-> & -> & _)".
+wp_rec. wp_pures. wp_apply (wp_handle_close Φ N _ _ _ cs); eauto.
+iIntros "%hc #wp_hc". wp_apply (@wp_cons val _ _ _ _ hc).
+iAssert ([∗ list] h ∈ (hc :: handlers), handler Φ _ _ cs N h)%I
+  as "#wp".
+{ rewrite /=; iSplit => //. eauto. }
+iClear "wp_hc". wp_bind (Conn.select _ _ _).
+iApply (wp_wand with "[inv conn rel clockS]").
+{ wp_apply (Conn.wp_select with "chan_c wp [$conn $rel $inv $clockS]").
+  by eauto. }
+iIntros "%res (%n0' & _ & #beg' & Hres)".
+iPoseProof (term_meta_agree with "beg beg'") as "<-".
+iDestruct "Hres" as "[(-> & Hres)|(-> & Hres)]".
+- iDestruct "Hres" as "(inv & conn & clockS & rel)". wp_pures.
+  wp_apply ("IH" with "[$inv $clockS $rel $conn]") => //.
+  do !iSplit => //. iExists n0. iSplit => //.
+  iPureIntro. lia.
+- iDestruct "Hres" as "(inv & clockS & rel)". wp_pures.
+  iApply "post". iExists (n0 + n1). iFrame. iModIntro.
+  iDestruct "clockS" as "[?|clockS]"; last by iRight.
+  iLeft. by iApply Conn.session_failed_failure.
 Qed.
 
 Lemma wp_close N c kI kR cs n :
-  channel c -∗
-  ctx N -∗
-  {{{ connected kI kR cs n ∗ client_token N kI kR cs }}}
+  {{{ channel c ∗ ctx N ∗ client_connected N kI kR cs n }}}
     close N c (repr cs)
-  {{{ RET #();
-      client_disconnected N kI kR n ∗
-      public (si_key cs) }}}.
+  {{{ RET #(); client_disconnected N kI kR n ∗ public (si_key cs) }}}.
 Proof.
-iIntros "#chan_c (_ & _ & #close & #ack & _)".
-iIntros "!> %Φ [conn token] post".
-iPoseProof (connected_keyE with "conn") as "[-> ->]".
-wp_lam. wp_pures.
-wp_apply (@wp_nil term).
-wp_apply (wp_write with "[//] [] [] [] [$]") => //.
-{ iRight. iModIntro. by eauto. }
+iIntros "%Φ (#chan_c & #ctx & conn) post".
+iDestruct "conn" as "(%n1 & %n0 & -> & conn & #beg & rel & clockC)".
+iPoseProof (Conn.connected_keyE with "conn") as "#(-> & -> & _)".
+wp_lam. wp_pures. wp_list.
+iPoseProof (Conn.connected_released_session with "conn") as "#p_k".
+iPoseProof (ctx_close with "[//]") as "#?".
+iPoseProof (ctx_ack_close with "[//]") as "#?".
+wp_apply (Conn.wp_write with "[//] [] [] [$conn clockC]") => //.
+{ rewrite /= public_TInt. by eauto. }
+{ iDestruct "clockC" as "[?|clockC]"; eauto.
+  iRight. iExists n0. by iFrame. }
 iIntros "conn". wp_pures.
-wp_apply (wp_read with "[//] [] [$]") => //.
-iIntros "%ts (conn & _ & #inv)".
-wp_pures.
-iAssert (|={⊤}=>
-  ⌜cs_role cs = Init⌝ ∗
-  client_disconnected N (si_init cs) (si_resp cs) n ∗
-  (compromised_session Init cs ∨ released (si_resp_share cs)))%I
-  with "[token]" as ">(%e_rl & dis & #relR)".
-{ iDestruct "token" as "(-> & #server & end)".
-  iDestruct "inv" as "[fail|[inv #rel]]".
-  { iModIntro. do !iSplit => //; eauto.
-    iLeft. by iApply session_failed_failure. }
-  iMod (escrowE with "inv end") as ">c1" => //.
-  iModIntro. iFrame. do !iSplit => //. by eauto. }
-iDestruct "conn" as "(% & % & _ & _ & _ & _ & #wf & rel & ts & _)".
-iDestruct "wf" as "(_ & _ & #sec & _)".
-iMod (release with "rel") as "#relI".
-rewrite /cs_share e_rl /=.
-wp_apply (wp_free with "[$]"). iIntros "_".
-iApply "post". iFrame.
-iDestruct "relR" as "[(_ & ? & _)|relR]"; eauto.
-iApply "sec". iSplit => //.
-Qed.
-
-Definition handler_loop_post φ skI skR cs n res : iProp :=
-  ⌜res = #true⌝ ∗ ∃ n', connected skI skR cs n' ∗ φ n'.
-
-Definition handler_correct φ skI skR cs handler : iProp :=
-  handler_correct_gen φ (handler_loop_post φ skI skR cs)
-           skI skR cs handler.
-
-Definition handler_loop_post_gen φ N skI skR cs n res : iProp :=
-  ⌜res = #true⌝ ∗
-    (∃ n', connected skI skR cs n' ∗ server_token N cs ∗ φ n') ∨
-  ⌜res = #false⌝ ∗
-    ∃ n', server_disconnected N skI skR n' ∗ φ n'.
-
-Lemma wp_handle_loop c N skI skR cs n φ ψ handlers :
-  channel c -∗
-  ([∗ list] handler ∈ handlers,
-    make_handler_post
-      (λ n, server_token N cs ∗ φ n)
-      (handler_loop_post_gen φ N skI skR cs)
-      skI skR cs handler) -∗
-  connected skI skR cs n -∗
-  server_token N cs -∗
-  φ n -∗
-  (∀ n', server_disconnected N skI skR n' ∗ φ n' -∗ ψ #()) -∗
-  WP handle_loop c (repr cs) (repr handlers) {{ ψ }}.
-Proof.
-iIntros "#chan_c #wps conn token inv post".
-iApply (wp_frame_wand with "post").
-iLöb as "IH" forall (n).
-iDestruct "conn" as "(%n1 & %n0 & -> & #beg & conn)".
-wp_rec. wp_pures. iCombine "token inv" as "inv".
-iPoseProof (wp_select_outer_body with "chan_c wps beg conn inv") as "wp".
-wp_bind (select_outer_body _ _ _). iApply (wp_wand with "wp").
-iIntros "% [(-> & %n' & conn & token & inv)|(-> & %n' & dis)]".
-- wp_pures. by iApply ("IH" with "conn token inv").
-- wp_pures. iModIntro. iIntros "post". by iApply "post".
-Qed.
-
-Lemma wp_handle
-  φ ψ (c : val) skI skR cs n N (handlers : list (namespace * expr)) :
-  channel c -∗
-  ctx N -∗
-  ([∗ list] handler ∈ handlers, handler_correct φ skI skR cs handler) -∗
-  connected skI skR cs n -∗
-  server_token N cs -∗
-  φ n -∗
-  (∀ n', server_disconnected N skI skR n' ∗ φ n' -∗ ψ #()) -∗
-  WP handle N c (repr cs) handlers {{ ψ }}.
-Proof.
-iIntros "#chan_c #ctx wps conn token inv post".
-rewrite handle_eq /handle_def.
-iAssert ([∗ list] handler ∈ handlers, handler_correct_gen
-           (λ n, server_token N cs ∗ φ n)
-           (handler_loop_post_gen φ N skI skR cs)
-           skI skR cs handler)%I with "[wps]" as "wps".
-{ iApply (big_sepL_impl with "wps").
-  iIntros "!> % % _ wp".
-  rewrite /handler_correct_gen.
-  iApply (wp_wand with "wp").
-  iIntros "%v_handler (%ψ' & #? & #wp)".
-  iExists ψ'. iSplit => //.
-  iIntros "!> %n' %ts !> %ψ'' (conn & (token & inv) & #p_ts & #inv_ts)".
-  iIntros "post". iApply ("wp" with "[$conn $inv]"); eauto.
-  iIntros "!> %res [(-> & conn & inv)|(%v & -> & -> & %n'' & conn & inv)]".
-  - iApply "post". iLeft. by iFrame.
-  - iApply "post". iRight. iExists _. iSplit => //.
-    iLeft. by iFrame. }
-iAssert (handler_correct_gen
-           (λ n, server_token N cs ∗ φ n)
-           (handler_loop_post_gen φ N skI skR cs)
-           skI skR cs (N.@"conn".@"close",
-             handle_close N c (repr cs)))%I as "wp_close".
-{ iPoseProof (ctx_close with "ctx") as "#?".
-  iPoseProof (ctx_ack_close with "ctx") as "#?".
-  rewrite /handler_correct_gen /handle_close. wp_pures.
-  iModIntro. iExists _. iSplit => //.
-  iIntros "!> %n' %ts !> %ψ' (conn & (token & inv) & _ & _) post". wp_pures.
-  iPoseProof (connected_keyE skI skR cs n' with "conn") as "%e".
-  iDestruct "conn" as "(%n1 & %n0 & -> & _ & conn)".
-  iAssert (⌜cs_role cs = Resp⌝)%I as "%e_rl".
-  { by iDestruct "token" as "[??]". }
-  iAssert (|==> (connected' skI skR cs true n1 n0 ∗
-             released (si_resp_share cs)))%I
-    with "[conn]" as ">[conn #rel]".
-  { iDestruct "conn" as "(<- & <- & ? & rel & ts & ?)".
-    iMod (release with "rel") as "#rel".
-    iModIntro. iFrame. rewrite /cs_share /= e_rl. by eauto. }
-  iAssert (|={⊤}=>
-    server_disconnected N skI skR (n1 + n0) ∗
-    (compromised_session Resp cs ∨
-     □ ack_close_pred N skI skR cs (n1 + n0) [TInt 0]))%I
-  with "[token]" as ">(dis & #?)".
-  { rewrite /server_disconnected.
-    case: e => -> ->.
-    iDestruct "token" as "[_ token]".
-    iDestruct "token" as "[#fail|(%n'' & c1 & c2)]".
-    { iModIntro. rewrite -session_failed_failure.
-      iSplit => //; eauto. }
-    iMod (clock_update N (n1 + n0) with "c1 c2") as "[c1 c2]".
-    iAssert (|={⊤}=> conn_closed N cs (n1 + n0))%I with "[c2]" as ">#?".
-    { iApply (escrowI with "c2"). iApply term_token_switch. }
-    iModIntro.
-    iFrame. iRight. iModIntro. by iSplit. }
-  wp_list. rewrite -e_rl.
-  wp_apply (wp_write' with "[//] [] [] [//] [$]") => //.
-  - by rewrite /= public_TInt.
-  iIntros "conn". wp_pures.
-  iDestruct "conn" as "(_ & _ & _ & _ & ts & _)".
-  wp_apply (wp_free with "[$]"). iIntros "_". wp_pures.
-  iModIntro. iApply "post". iRight. iExists _. iSplit => //.
-  iRight. iSplit => //. iExists (n1 + n0). by iFrame. }
-iPoseProof (wp_make_handlers with "wps") as "wp".
-wp_bind (make_handlers _). iApply (wp_wand with "wp").
-iIntros "%res (%handlers' & -> & #wps')".
-wp_pures. rewrite !subst_make_handler /=.
-iPoseProof (wp_make_handler with "wp_close") as "{wp_close} wp_close".
-wp_bind (make_handler _). iApply (wp_wand with "wp_close").
-iIntros "%v_close {wp_close} #wp_close".
-wp_bind (_ :: _)%E.
-wp_apply (@wp_cons val _ _ _ _ v_close).
-iApply (wp_handle_loop with "[//] [] conn token inv").
-{ by rewrite /=; iSplit => //. }
-by [].
+wp_apply (Conn.wp_read with "[//] [] [$]") => //.
+iIntros "%ts (conn & rel & _ & inv)".
+wp_pures. iMod (release with "rel") as "#relC".
+wp_apply (Conn.wp_free with "[$conn]"). iIntros "_".
+iApply "post". iDestruct "inv" as "[#comp|inv]".
+- iSplit.
+  + iLeft. by iApply Conn.session_failed_failure.
+  + by iDestruct "comp" as "(_ & ? & _)".
+- iDestruct "inv" as "(%n0' & #beg' & clockC & #relS)".
+  iPoseProof (term_meta_agree with "beg beg'") as "<-".
+  iSplit.
+  + by iRight.
+  + iApply "p_k". by iSplit.
 Qed.
 
 End Proofs.
