store/client_proofs/create.v
@@ -5,7 +5,7 @@ From iris.algebra Require Import agree auth csum gset gmap excl frac.
 From iris.algebra Require Import max_prefix_list.
 From iris.heap_lang Require Import notation proofmode.
 From cryptis Require Import lib term gmeta nown cryptis.
-From cryptis Require Import primitives tactics role rpc.
+From cryptis Require Import primitives tactics role conn rpc.
 From cryptis.store Require Import impl shared db.
 
 Set Implicit Arguments.
@@ -14,12 +14,12 @@ Unset Printing Implicit Defensive.
 
 Section Verif.
 
-Context `{!cryptisGS Σ, !heapGS Σ, !storeGS Σ}.
+Context `{!cryptisGS Σ, !heapGS Σ, !Conn.connGS Σ, !storeGS Σ}.
 Notation iProp := (iProp Σ).
 
 Context `{!storeG Σ}.
 
-Implicit Types (cs : RPC.state).
+Implicit Types (cs : Conn.state).
 Implicit Types kI kR kS t : term.
 Implicit Types n : nat.
 Implicit Types γ : gname.
@@ -29,6 +29,7 @@ Variable N : namespace.
 
 Lemma wp_client_create c kI kR cs t1 t2 :
   channel c -∗
+  cryptis_ctx -∗
   store_ctx N -∗
   public t1 -∗
   public t2 -∗
@@ -39,22 +40,16 @@ Lemma wp_client_create c kI kR cs t1 t2 :
       db_connected N kI kR cs ∗
       rem_mapsto N kI kR t1 t2 }}}.
 Proof.
-iIntros "#chan_c (_ & _ & _ & _ & #create & #ack & _) #p_t1 #p_t2".
+iIntros "#chan_c #? (_ & _ & #create & #ctx) #p_t1 #p_t2".
 iIntros "!> %Φ [client free] post".
-iDestruct "client"
-  as "(%n & %db & conn & version & #db_at & state & token)".
+iDestruct "client" as "(%n & %db & conn & version & #db_at & state)".
 iMod (DB.create_client t1 t2 with "version db_at state free")
   as "(#create_at & version & #db_at' & state & mapsto)".
 wp_lam. wp_pures. wp_list.
-wp_apply (RPC.wp_write with "[//] [] [] [] [$]") => //.
-- by rewrite /=; eauto.
-- iRight. iExists _, _. by eauto.
-iIntros "conn". wp_pures.
-wp_apply (RPC.wp_read with "[//] [] [$]") => //.
-- iIntros "%ts (conn & _ & _)". wp_pures.
-wp_apply (RPC.wp_tick with "[$]").
-iIntros "conn". iApply "post".
-by iFrame.
+wp_apply (RPC.wp_call with "[$conn]").
+{ do !iSplit => //. iRight. iExists _, _. by eauto. }
+iIntros "%ts (conn & _ & _)". wp_pures.
+iApply "post". by iFrame.
 Qed.
 
 End Verif.
