store/client_proofs/load.v
@@ -7,7 +7,7 @@ From iris.base_logic Require Import invariants.
 From iris.heap_lang Require Import notation proofmode.
 From cryptis Require Import lib term gmeta nown cryptis.
 From cryptis Require Import primitives tactics.
-From cryptis Require Import role iso_dh rpc.
+From cryptis Require Import role iso_dh conn rpc.
 From cryptis.store Require Import impl shared db.
 
 Set Implicit Arguments.
@@ -16,7 +16,7 @@ Unset Printing Implicit Defensive.
 
 Section Verif.
 
-Context `{!cryptisGS Σ, !heapGS Σ, !storeGS Σ}.
+Context `{!cryptisGS Σ, !heapGS Σ, !Conn.connGS Σ, !storeGS Σ}.
 Notation iProp := (iProp Σ).
 
 Context `{!storeG Σ}.
@@ -30,6 +30,7 @@ Variable N : namespace.
 
 Lemma wp_client_load c kI kR cs t1 t2 :
   channel c -∗
+  cryptis_ctx -∗
   store_ctx N -∗
   public t1 -∗
   {{{ db_connected N kI kR cs ∗
@@ -41,28 +42,22 @@ Lemma wp_client_load c kI kR cs t1 t2 :
       public t2' ∗
       (compromised_session Init cs ∨ ⌜t2' = t2⌝) }}}.
 Proof.
-iIntros "#chan_c #ctx #p_t1 !> %Φ [client mapsto] post".
-iDestruct "client"
-  as "(%n & %db & conn & version & #db_at & state & token)".
-iAssert (⌜RPC.cs_role cs = Init⌝)%I as "%e_rl".
-{ by iDestruct "token" as "(? & ?)". }
+iIntros "#chan_c #? #ctx #p_t1 !> %Φ [client mapsto] post".
+iDestruct "client" as "(%n & %db & conn & version & #db_at & state)".
 wp_lam; wp_pures. wp_list.
 iMod (DB.load_client t1 with "version db_at")
   as "(#load_at & version & db)".
-iDestruct "ctx" as "(_ & _ & load & ack_load & _)".
-wp_apply (RPC.wp_write with "chan_c load [] [] [$]").
-- by rewrite /=; eauto.
-- iRight. iIntros "!>". iExists _. by eauto.
-iIntros "conn". wp_pures.
-wp_apply (RPC.wp_read with "chan_c [//] [$]").
-iIntros "%ts (conn & #p_ts & #inv_ts)". wp_pures.
-wp_apply (RPC.wp_tick with "conn"). iIntros "conn".
-rewrite [repr_list ts]repr_listE.
+iDestruct "ctx" as "(_ & load & _ & ctx)".
+wp_apply (RPC.wp_call with "[$conn]").
+{ do 4!iSplit => //=; first by eauto.
+  iSplit => //. iRight. iExists _. by eauto. }
+iIntros "%ts' (conn & #inv_ts & p_ts)". wp_pures.
+rewrite [repr_list ts']repr_listE.
 iDestruct "inv_ts" as "[fail|inv_ts]".
-- wp_pures. case: ts => [|t ts]; wp_pures.
-  + iApply "post". iFrame. rewrite public_TInt e_rl. by eauto.
+- wp_pures. case: ts' => [|t ts]; wp_pures.
+  + iApply "post". iFrame. rewrite public_TInt. by eauto.
   + rewrite /=. iDestruct "p_ts" as "[p_t _]".
-    iApply "post". iFrame. rewrite e_rl. by eauto.
+    iApply "post". iFrame. by eauto.
 iDestruct "inv_ts" as "(%t1' & %t2' & -> & load_at' & stored_at)".
 iPoseProof (DB.op_at_agree with "load_at load_at'") as "%e".
 case: e => <-.
