store/client_proofs/store.v
@@ -5,7 +5,7 @@ From iris.algebra Require Import agree auth csum gset gmap excl frac.
 From iris.algebra Require Import max_prefix_list.
 From iris.heap_lang Require Import notation proofmode.
 From cryptis Require Import lib term cryptis primitives tactics.
-From cryptis Require Import role rpc.
+From cryptis Require Import role conn rpc.
 From cryptis.store Require Import impl shared db.
 
 Set Implicit Arguments.
@@ -14,12 +14,12 @@ Unset Printing Implicit Defensive.
 
 Section Verif.
 
-Context `{!cryptisGS Σ, !heapGS Σ, !storeGS Σ}.
+Context `{!cryptisGS Σ, !heapGS Σ, !Conn.connGS Σ, !storeGS Σ}.
 Notation iProp := (iProp Σ).
 
 Context `{!storeG Σ}.
 
-Implicit Types (cs : RPC.state).
+Implicit Types (cs : Conn.state).
 Implicit Types kI kR kS t : term.
 Implicit Types n : nat.
 Implicit Types γ : gname.
@@ -29,6 +29,7 @@ Variable N : namespace.
 
 Lemma wp_client_store c kI kR cs t1 t2 t2' :
   channel c -∗
+  cryptis_ctx -∗
   store_ctx N -∗
   public t1 -∗
   public t2' -∗
@@ -36,22 +37,18 @@ Lemma wp_client_store c kI kR cs t1 t2 t2' :
     Client.store N c (repr cs) t1 t2'
   {{{ RET #(); db_connected N kI kR cs ∗ rem_mapsto N kI kR t1 t2' }}}.
 Proof.
-iIntros "#chan_c #ctx #p_t1 #p_t2 !> %Φ [client mapsto] post".
-iDestruct "client"
-  as "(%n & %db & conn & version & #db_at & state & token)".
+iIntros "#chan_c #? #ctx #p_t1 #p_t2 !> %Φ [client mapsto] post".
+iDestruct "client" as "(%n & %db & conn & version & #db_at & state)".
 wp_lam. wp_pures. wp_list.
 iMod (DB.store_client t2' with "version db_at state mapsto")
   as "(version & #db_at' & #store_at & state & mapsto)".
-wp_apply (RPC.wp_write with "[//] [] [] [] [$]").
-- by iApply store_ctx_store.
-- rewrite /=; eauto.
-- iRight. by iExists t1, t2'; eauto.
-iIntros "conn". wp_pures.
-wp_apply (RPC.wp_read with "[//] [] [$]").
-- by iApply store_ctx_ack_store.
-iIntros "%ts [conn _]". wp_pures.
-wp_apply (RPC.wp_tick with "[$]"). iIntros "conn".
-iApply "post". by iFrame.
+iPoseProof (store_ctx_store with "[//]") as "?".
+iPoseProof (store_ctx_rpc_ctx with "[//]") as "?".
+wp_apply (RPC.wp_call with "[$conn]").
+{ do 4!iSplit => //=; first by eauto.
+  iSplit => //. iRight. iExists _, _. by eauto. }
+iIntros "%ts' (conn & _ & _)". wp_pures. iApply "post".
+by iFrame.
 Qed.
 
 End Verif.
