store/server_proofs/create.v
@@ -5,7 +5,7 @@ From iris.algebra Require Import agree auth csum gset gmap excl frac.
 From iris.algebra Require Import max_prefix_list.
 From iris.heap_lang Require Import notation proofmode.
 From cryptis Require Import lib term cryptis primitives tactics.
-From cryptis Require Import role iso_dh rpc.
+From cryptis Require Import role iso_dh conn rpc.
 From cryptis.store Require Import impl shared alist db.
 
 Set Implicit Arguments.
@@ -14,10 +14,10 @@ Unset Printing Implicit Defensive.
 
 Section Verif.
 
-Context `{!cryptisGS Σ, !heapGS Σ, !storeGS Σ}.
+Context `{!cryptisGS Σ, !heapGS Σ, !Conn.connGS Σ, !storeGS Σ}.
 Notation iProp := (iProp Σ).
 
-Implicit Types (cs : RPC.state).
+Implicit Types (cs : Conn.state).
 Implicit Types kI kR kS t : term.
 Implicit Types n : nat.
 Implicit Types γ : gname.
@@ -27,33 +27,31 @@ Variable N : namespace.
 
 Ltac failure := iLeft; iFrame; eauto.
 
-Lemma wp_server_handle_create c kI kR cs vdb :
-  RPC.cs_role cs = Resp →
-  channel c -∗
-  store_ctx N -∗
-  RPC.handler_correct
-    (server_db_connected' N kI kR cs vdb)
-    kI kR cs
-    (N.@"create", Server.handle_create N c (repr cs) vdb).
+Lemma wp_server_handle_create c kI kR cs (vdb : val) :
+  {{{ channel c ∗ cryptis_ctx ∗ store_ctx N }}}
+    RPC.handle N "create" c (Server.handle_create c (repr cs) vdb)
+  {{{ h, RET h; server_handler N kI kR cs vdb h }}}.
 Proof.
-iIntros "%e_rl #chan_c #ctx".
-iPoseProof (store_ctx_create with "ctx") as "?".
-iPoseProof (store_ctx_ack_create with "ctx") as "?".
-rewrite /RPC.handler_correct /RPC.handler_correct_gen.
-wp_lam. wp_pures. iModIntro. iExists _. iSplit => //.
-iIntros "!> %n %ts !> %Φ (conn & db & #p_ts & #inv_ts) post".
-wp_pures. iApply (wp_wand with "[conn db] post").
-iDestruct "db" as "(%db & #p_db & db & #db_at)".
-wp_list_match => [t1 t2 ->| _]; wp_pures; last by failure.
+iIntros "%Φ (#chan_c & #ctx & #ctx') post".
+iPoseProof (store_ctx_create with "[//]") as "?".
+iPoseProof (store_ctx_rpc_ctx with "[//]") as "?".
+wp_lam. wp_pures.
+wp_apply RPC.wp_handle; last by eauto.
+do 3!iSplit => //. clear Φ.
+iIntros "!> %n %ts !> %Φ (#p_ts & #inv_ts & %db & #p_db & db & #db_at) post".
+wp_list_match => [t1 t2 ->| ?]; wp_pures; last first.
+{ iApply ("post" $! None). iFrame.
+  iDestruct "inv_ts" as "[fail|inv_ts]"; eauto.
+  by iDestruct "inv_ts" as "(% & % & -> & ?)". }
+rewrite /=. iDestruct "p_ts" as "(p_t1 & p_t2 & _)".
 wp_bind (SAList.find _ _). iApply (SAList.wp_find with "db") => //.
 iIntros "!> db". rewrite lookup_fmap.
 wp_bind (match: _ with InjL <> => _ | InjR <> => _ end)%E.
-iApply (wp_frame_wand with "conn").
 iAssert (compromised_session Resp cs ∨
            DB.db_at kI (N.@"client".@kR.@"db")
              (S n) (DB.op_app db (Create t1 t2)))%I
   as "#db_at'".
-{ rewrite e_rl. iDestruct "inv_ts" as "[?|inv_ts]"; eauto.
+{ iDestruct "inv_ts" as "[?|inv_ts]"; eauto.
   iDestruct "inv_ts" as "(%t1' & %t2' & %e & create_at)".
   case: e => <- <-.
   iDestruct "db_at" as "[?|db_at]"; eauto.
@@ -71,22 +69,14 @@ iApply (wp_wand _ _ _ (λ v,
   wp_pures.
   iFrame. iExists true. rewrite /= db_t1.
   iModIntro. do !iSplit => //.
-  iDestruct "p_ts" as "(? & ? & _)".
   by iApply public_db_insert. }
-iIntros "% (%b & -> & db) conn".
+iIntros "% (%b & -> & db)".
 wp_pures.
 wp_bind (tint _). iApply wp_tint.
 wp_list.
 wp_pures.
-wp_apply (RPC.wp_write with "[//] [] [] [] [$]") => //.
-- rewrite /= public_TInt. iDestruct "p_ts" as "(? & ? & _)".
-  by eauto.
-- by iRight.
-iIntros "conn". wp_pures.
-wp_apply (RPC.wp_tick with "[$]"). iIntros "conn".
-wp_pures.
-iModIntro. iRight. iExists _. iSplit => //.
-iSplit => //. iExists (S n). by iFrame.
+iApply ("post" $! (Some _)).
+iModIntro. rewrite /= public_TInt. by iSplit; eauto.
 Qed.
 
 End Verif.
