store/server_proofs/load.v
@@ -6,7 +6,7 @@ From iris.algebra Require Import max_prefix_list.
 From iris.heap_lang Require Import notation proofmode.
 From cryptis Require Import lib term gmeta nown.
 From cryptis Require Import cryptis primitives tactics.
-From cryptis Require Import role rpc.
+From cryptis Require Import role conn rpc.
 From cryptis.store Require Import impl shared alist db.
 
 Set Implicit Arguments.
@@ -15,12 +15,10 @@ Unset Printing Implicit Defensive.
 
 Section Verif.
 
-Context `{!cryptisGS Σ, !heapGS Σ, !storeGS Σ}.
+Context `{!cryptisGS Σ, !heapGS Σ, !Conn.connGS Σ, !storeGS Σ}.
 Notation iProp := (iProp Σ).
 
-Context `{!storeGS Σ}.
-
-Implicit Types (cs : RPC.state).
+Implicit Types (cs : Conn.state).
 Implicit Types skI skR kS t : term.
 Implicit Types n : nat.
 Implicit Types γ : gname.
@@ -30,41 +28,44 @@ Variable N : namespace.
 
 Ltac failure := iLeft; iFrame; eauto.
 
-Lemma wp_server_handle_load c skI skR cs vdb :
-  RPC.cs_role cs = Resp →
-  channel c -∗
-  store_ctx N -∗
-  RPC.handler_correct
-    (server_db_connected' N skI skR cs vdb)
-    skI skR cs
-    (N.@"load", Server.handle_load N c (repr cs) vdb).
+Lemma wp_server_handle_load c skI skR cs (vdb : val) :
+  {{{ channel c ∗ cryptis_ctx ∗ store_ctx N  }}}
+    RPC.handle N "load" c (Server.handle_load c (repr cs) vdb)
+  {{{ h, RET h; server_handler N skI skR cs vdb h }}}.
 Proof.
-iIntros "%e_rl #chan_c #ctx".
+iIntros "%Φ (#chan_c & #? & #ctx) post".
 iPoseProof (store_ctx_load with "ctx") as "?".
-iPoseProof (store_ctx_ack_load with "ctx") as "?".
-rewrite /RPC.handler_correct /= /RPC.handler_correct_gen.
-wp_lam; wp_pures. iModIntro. iExists _. iSplit => //.
-iIntros "!> %n %ts !> %Φ (conn & db & #p_ts & #inv_ts) post".
-wp_pures.
-iApply (wp_wand with "[conn db] post").
-iDestruct "db" as "(%db & #p_db & db & #db_at)".
-wp_pures.
-wp_list_match => [t1 ->| _]; wp_pures; last by failure.
+iPoseProof (store_ctx_rpc_ctx with "ctx") as "?".
+wp_lam; wp_pures.
+wp_apply RPC.wp_handle; last by eauto.
+do 3!iSplit => //. clear Φ.
+iIntros "!> %n %ts !> %Φ (#p_ts & #inv_ts & %db & #p_db & db & #db_at) post".
+wp_pures. wp_list_match => [t1 ->| ?]; wp_pures; last first.
+{ iDestruct "inv_ts" as "[fail|(% & -> & ?)]" => //.
+  iApply ("post" $! None).
+  iModIntro. rewrite /=. iSplit; eauto. iFrame.
+  iSplit; eauto. }
 wp_bind (SAList.find _ _). iApply (SAList.wp_find with "db") => //.
 iIntros "!> db". rewrite lookup_fmap.
-case db_t1: (db !! t1) => [t2|]; wp_pures; last by failure.
-wp_list.
-rewrite -e_rl.
-iPoseProof (ack_load_predI with "inv_ts db_at") as "[? #?]" => //.
-wp_apply (RPC.wp_write with "[//] [] [] [] [$]") => //.
-- rewrite /public_db big_sepM_forall.
-  iDestruct ("p_db" $! t1 t2 with "[//]") as "[??]".
-  by rewrite /=; eauto.
-iIntros "conn". wp_pures.
-wp_apply (RPC.wp_tick with "conn"). iIntros "conn". wp_pures.
-iModIntro. iRight. iExists _. iSplit => //.
-iSplit => //. iExists (S n). iFrame.
-rewrite e_rl. by iSplit => //.
+case db_t1: (db !! t1) => [t2|]; wp_pures; last first.
+{ iApply ("post" $! None). iFrame. iModIntro. iSplit => //.
+  iDestruct "db_at" as "[fail|db_at]"; eauto.
+  iDestruct "inv_ts" as "[fail|(% & %e & load_at)]"; eauto.
+  iRight. iApply (DB.db_at_op_at with "db_at load_at"). }
+wp_list. wp_pures. iModIntro.
+iApply ("post" $! (Some _)). iFrame. do !iSplit; eauto.
+- rewrite /public_db big_sepM_forall /=.
+  by iDestruct ("p_db" $! t1 t2 with "[//]") as "[??]".
+- iDestruct "inv_ts" as "[fail|(% & %e & load_at)]"; eauto.
+  case: e => <-.
+  iDestruct "db_at" as "[fail|db_at]"; eauto.
+  iRight. iExists t1, t2. do 2!iSplit => //; eauto.
+  iApply DB.load_at_stored_at; eauto.
+  iApply DB.stored_atI; eauto.
+- iDestruct "inv_ts" as "[fail|(% & %e & load_at)]"; eauto.
+  case: e => <-.
+  iDestruct "db_at" as "[fail|db_at]"; eauto.
+  iRight. iApply (DB.db_at_op_at with "db_at load_at").
 Qed.
 
 End Verif.
