store/server_proofs/store.v
@@ -5,7 +5,7 @@ From iris.algebra Require Import agree auth csum gset gmap excl frac.
 From iris.algebra Require Import max_prefix_list.
 From iris.heap_lang Require Import notation proofmode.
 From cryptis Require Import lib term cryptis primitives tactics.
-From cryptis Require Import role rpc.
+From cryptis Require Import role conn rpc.
 From cryptis.store Require Import impl shared alist db.
 
 Set Implicit Arguments.
@@ -14,12 +14,12 @@ Unset Printing Implicit Defensive.
 
 Section Verif.
 
-Context `{!cryptisGS Σ, !heapGS Σ}.
+Context `{!cryptisGS Σ, !heapGS Σ, !Conn.connGS Σ}.
 Notation iProp := (iProp Σ).
 
 Context `{!storeGS Σ}.
 
-Implicit Types (cs : RPC.state).
+Implicit Types (cs : Conn.state).
 Implicit Types kI kR kS t : term.
 Implicit Types n : nat.
 Implicit Types γ : gname.
@@ -27,43 +27,34 @@ Implicit Types v : val.
 
 Variable N : namespace.
 
-Ltac failure := iLeft; iFrame.
-
-Lemma wp_server_handle_store c kI kR cs vdb :
-  RPC.cs_role cs = Resp →
-  channel c -∗
-  store_ctx N -∗
-  RPC.handler_correct
-    (server_db_connected' N kI kR cs vdb)
-    kI kR cs
-    (N.@"store", Server.handle_store N c (repr cs) vdb).
+Lemma wp_server_handle_store c kI kR cs (vdb : val) :
+  {{{ channel c ∗ cryptis_ctx ∗ store_ctx N }}}
+    RPC.handle N "store" c (Server.handle_store c (repr cs) vdb)
+  {{{ h, RET h; server_handler N kI kR cs vdb h }}}.
 Proof.
-iIntros "%e_rl #chan_c #ctx".
+iIntros "%Φ (#chan_c & #? & #ctx) post".
 iPoseProof (store_ctx_store with "ctx") as "?".
-iPoseProof (store_ctx_ack_store with "ctx") as "?".
-rewrite /RPC.handler_correct /= /RPC.handler_correct_gen.
-wp_lam; wp_pures. iModIntro. iExists _. iSplit => //.
-iIntros "!> %n %ts !> %Φ (conn & db & #p_ts & #inv_m) post".
-wp_pures. iApply (wp_wand with "[conn db] post").
-wp_list_match => [t1 t2 ->|_]; wp_pures; last by failure.
-iDestruct "db" as "(%db & #p_db & db & #db_at)".
+iPoseProof (store_ctx_rpc_ctx with "ctx") as "?".
+wp_lam; wp_pures. wp_apply RPC.wp_handle; last by eauto.
+do 3!iSplit => //. clear Φ.
+iIntros "!> %n %ts !> %Φ (#p_ts & #inv_ts & %db & #p_db & db & #db_at) post".
+wp_pures.
+wp_list_match => [t1 t2 ->|?]; wp_pures; last first.
+{ iDestruct "inv_ts" as "[fail|inv_ts]"; last first.
+  { by iDestruct "inv_ts" as "(% & % & -> & ?)". }
+  wp_list. iApply ("post" $! None). iModIntro. iFrame.
+  rewrite /=. iSplit; eauto. }
 wp_bind (SAList.insert _ _ _).
 iApply (SAList.wp_insert with "db").
 iIntros "!> db". rewrite -fmap_insert.
-wp_pures.
-wp_apply (@wp_nil term).
-wp_apply (RPC.wp_write with "[] [] [] [] [$]") => //.
-{ iRight. by eauto. }
-iIntros "conn". wp_pures. 
-wp_apply (RPC.wp_tick with "[$]"). iIntros "conn". wp_pures.
-iModIntro. iRight. iExists _. iSplit => //.
-iSplit => //. iExists (S n). iFrame.
+wp_pures. wp_list. wp_pures. iApply ("post" $! (Some _)).
 rewrite /=.
+iModIntro. iSplit; first by eauto.
+iFrame.
 iDestruct "p_ts" as "(p_t1 & p_t2 & _)".
 iSplit; first by iApply public_db_insert.
-rewrite e_rl.
-iDestruct "inv_m" as "[fail|inv_m]"; eauto.
-iDestruct "inv_m" as "(%t1' & %t2' & %e & store_at)".
+iDestruct "inv_ts" as "[fail|inv_ts]"; eauto.
+iDestruct "inv_ts" as "(%t1' & %t2' & %e & store_at)".
 case: e => <- <-.
 iDestruct "db_at" as "[fail|db_at]"; eauto.
 iRight. iApply (DB.db_at_store_at with "db_at store_at").
